proper context for basic Simplifier operations: rewrite_rule, rewrite_goals_rule, rewrite_goals_tac etc.; clarified tool context in some boundary cases;

src/HOL/Decision_Procs/Parametric_Ferrante_Rackoff.thy
@@ -2920,7 +2920,7 @@ structure Parametric_Ferrante_Rackoff =
 struct
 
 fun tactic ctxt alternative T ps = 
-  Object_Logic.full_atomize_tac
+  Object_Logic.full_atomize_tac ctxt
   THEN' CSUBGOAL (fn (g, i) =>
     let
       val th = frpar_oracle (ctxt, alternative, T, ps, g)
