src/Sequents/S43.thy
@@ -90,8 +90,8 @@ structure S43_Prover = Modal_ProverFun
 
 
 method_setup S43_solve = {*
-  Scan.succeed (K (SIMPLE_METHOD
-    (S43_Prover.solve_tac 2 ORELSE S43_Prover.solve_tac 3)))
+  Scan.succeed (fn ctxt => SIMPLE_METHOD
+    (S43_Prover.solve_tac ctxt 2 ORELSE S43_Prover.solve_tac ctxt 3))
 *}
 
 
